safechecker/theories/clauses.v
@@ -1,0 +1,330 @@
+From Coq Require Import Program RelationClasses Morphisms.
+From Coq Require Import OrderedTypeAlt OrderedTypeEx MSetList MSetAVL MSetFacts MSetProperties MSetDecide.
+From MetaCoq.Template Require Import utils Universes.
+From Equations Require Import Equations.
+
+Definition clause : Type := nonEmptyLevelExprSet × LevelExpr.t.
+Module Clause.
+  Definition t := clause.
+
+  Definition eq : t -> t -> Prop := eq.
+
+  Definition eq_equiv : RelationClasses.Equivalence eq := _.
+
+  Inductive lt_ : t -> t -> Prop :=
+  | lt_clause1 l e e' : LevelExpr.lt e e' -> lt_ (l, e) (l, e')
+  | lt_clause2 l l' b b' : LevelExprSet.lt l.(t_set) l'.(t_set) -> lt_ (l, b) (l', b').
+
+  Definition lt := lt_.
+
+  Global Instance lt_strorder : RelationClasses.StrictOrder lt.
+  Proof.
+    constructor.
+    - intros x X; inversion X; subst. now eapply LevelExpr.lt_strorder in H1.
+      eapply LevelExprSet.lt_strorder; eassumption.
+    - intros x y z X1 X2; invs X1; invs X2; constructor; tea.
+      etransitivity; tea.
+      etransitivity; tea.
+  Qed.
+
+  Definition lt_compat : Proper (Logic.eq ==> Logic.eq ==> iff) lt.
+    intros x x' H1 y y' H2. unfold lt. subst. reflexivity.
+  Qed.
+
+  Definition compare (x y : t) : comparison :=
+    match x, y with
+    | (l1, b1), (l2, b2) =>
+      match LevelExprSet.compare l1.(t_set) l2.(t_set) with
+      | Eq => LevelExpr.compare b1 b2
+      | x => x
+      end
+    end.
+
+  Definition compare_spec :
+    forall x y : t, CompareSpec (x = y) (lt x y) (lt y x) (compare x y).
+  Proof.
+    intros [? ?] [? ?]; cbn; repeat constructor.
+    destruct (LevelExprSet.compare_spec n n0); repeat constructor; tas.
+    eapply LevelExprSet.eq_leibniz in H. apply NonEmptySetFacts.eq_univ in H.
+    subst. cbn in *.
+    destruct (LevelExpr.compare_spec t0 t1); repeat constructor; tas. now subst.
+  Qed.
+
+  Global Instance reflect_t : ReflectEq t := reflect_prod _ _ .
+
+  Definition eq_dec : forall (l1 l2 : t), {l1 = l2} + {l1 <> l2} := Classes.eq_dec.
+
+  Definition eq_leibniz (x y : t) : eq x y -> x = y := id.
+End Clause.
+
+Module Clauses := MSetList.MakeWithLeibniz Clause.
+Module ClausesFact := WFactsOn Clause Clauses.
+Module ClausesProp := WPropertiesOn Clause Clauses.
+
+Definition clauses := Clauses.t.
+
+Module MoreLevel.
+
+  Include Level.
+
+  Lemma compare_sym : forall x y : t, (compare y x) = CompOpp (compare x y).
+  Proof.
+    induction x; destruct y; simpl; auto.
+    apply StringOT.compare_sym.
+    apply PeanoNat.Nat.compare_antisym.
+  Qed.
+  
+  Lemma eq_refl x : eq x x.
+  Proof. red. reflexivity. Qed.
+
+  Lemma eq_sym x y : eq x y -> eq y x.
+  Proof. unfold eq. apply symmetry. Qed.
+ 
+  Lemma eq_trans x y z : eq x y -> eq y z -> eq x z.
+  Proof. unfold eq. apply transitivity. Qed.
+
+  Infix "?=" := compare.
+
+  Lemma compare_trans :
+    forall c (x y z : t), (x?=y) = c -> (y?=z) = c -> (x?=z) = c.
+  Proof.
+    intros c x y z.
+    destruct (compare_spec x y) => <-; subst.
+    destruct (compare_spec y z); auto.
+    destruct (compare_spec y z); auto; try congruence.
+    destruct (compare_spec x z); auto; try congruence.
+    subst. elimtype False. eapply (irreflexivity (A:=t)). etransitivity; [exact H|exact H0].
+    elimtype False. eapply (irreflexivity (A:=t)). etransitivity; [exact H|]. 
+    eapply transitivity; [exact H0|exact H1].
+    destruct (compare_spec y z); auto; try congruence.
+    destruct (compare_spec x z); auto; try congruence.
+    subst. elimtype False. eapply (irreflexivity (A:=t)). etransitivity; [exact H|exact H0].
+    elimtype False. eapply (irreflexivity (A:=t)). etransitivity; [exact H|]. 
+    eapply transitivity; [exact H1|exact H0].
+  Qed.
+
+End MoreLevel.
+
+Module LevelOT := OrderedType_from_Alt MoreLevel.
+Module LevelMap := FMapAVL.Make LevelOT.
+Module LevelMapFact := FMapFacts.WProperties LevelMap.
+
+Definition model := LevelMap.t nat.
+
+Definition premise (cl : clause) := fst cl.
+
+Definition concl (cl : clause) := snd cl.
+
+Definition matches_clause (cl : clause) (m : model) :=
+  LevelExprSet.exists_ (fun '(l, k) => LevelMap.find l m == Some k) (premise cl).
+
+Definition update_model (m : model) (w : LevelSet.t) (e : LevelExpr.t) : 
+  option (LevelSet.t * model) :=
+  let (l, k) := e in
+  match LevelMap.find l m with
+  | Some k' => if k' <? k then Some (LevelSet.add l w, LevelMap.add l k m) else None
+  | None => None
+  end.
+
+Definition new_atoms (cls : clauses) (m : model) (w : LevelSet.t) : option (LevelSet.t * model) :=
+  Clauses.fold
+    (fun cl acc => 
+      if matches_clause cl m then 
+        match update_model m w (concl cl) with
+        | Some v' => Some v'
+        | None => acc
+        end
+      else acc)
+    cls None.
+
+(* Variant model_check :=
+  | Satisfiable
+  | Unsatisfiable (cls : clauses). *)
+
+Definition satisfiable_atom (m : model) (atom : Level.t * nat) : bool :=
+  let '(l, k) := atom in
+  match LevelMap.find l m with
+  | Some val => k <=? val
+  | None => false
+  end.
+  
+Definition level_value (m : model) (level : Level.t) : nat :=
+  match LevelMap.find level m with
+  | Some val => val
+  | None => 0
+  end.
+
+#[program] 
+Definition choose (l : nonEmptyLevelExprSet) : LevelExpr.t :=
+  match LevelExprSet.choose l with
+  | Some l => l
+  | None => !%prg
+  end.
+
+Next Obligation.
+  symmetry in Heq_anonymous.
+  eapply LevelExprSet.choose_spec2, LevelExprSetFact.is_empty_1 in Heq_anonymous.
+  destruct l. cbn in *. congruence.    
+Qed.
+
+Definition min_atom_value (m : model) (atom : LevelExpr.t) :=
+  let '(l, k) := atom in
+  (Z.of_nat (level_value m l) - Z.of_nat k)%Z.
+
+Definition min_premise (m : model) (l : nonEmptyLevelExprSet) : Z :=
+  LevelExprSet.fold (fun atom min => Z.min (min_atom_value m atom) min) l 
+   (min_atom_value m (choose l)).
+
+Definition satisfiable_premise (m : model) (l : nonEmptyLevelExprSet) :=
+  LevelExprSet.exists_ (satisfiable_atom m) l.
+
+Definition valid_clause (m : model) (cl : clause) :=
+  implb (satisfiable_premise m (premise cl)) (satisfiable_atom m (concl cl)).
+
+Definition is_model (cls : clauses) (m : model) : bool :=
+  Clauses.for_all (valid_clause m) cls.
+
+Definition update_map l k v :=
+  match LevelMap.find l v with
+  | Some k' => LevelMap.add l (Nat.max k k') v
+  | None => LevelMap.add l k v
+  end. 
+
+Definition update_value (wv : LevelSet.t × model) (cl : clause) : option (LevelSet.t × model) :=
+  let (w, v) := wv in
+  let k0 := min_premise v (premise cl) in
+  (* cl holds vacuously as the premise doesn't hold *)
+  if (k0 <? 0)%Z then None
+  else 
+    (* The premise does hold *)
+    let (l, k) := concl cl in
+    (* Does the conclusion also hold ? *)
+    if k + Z.to_nat k0 <=? level_value v l then None
+    else 
+      (* The conclusion doesn't hold, we need to set it higher *)
+      (* let (w, v) := cur in *)
+      Some (LevelSet.add l w, update_map l (k + Z.to_nat k0) v).
+
+Definition check_model (cls : clauses) (wv : LevelSet.t × model) : 
+    option (LevelSet.t × model) :=
+  Clauses.fold
+    (fun cl acc => 
+      let cur := match acc with None => wv | Some acc => acc end in
+      match update_value cur cl with 
+      | Some acc => Some acc
+      | None => acc
+      end)
+    cls None.
+
+Inductive result :=
+  | Loop
+  | Unsatisfiable (w : LevelSet.t) (m : model)
+  | Model (w : LevelSet.t) (m : model).
+
+#[bypass_check(guard)]
+Fixpoint forward (V : LevelSet.t) (cls : clauses) (m : model) (w : LevelSet.t) { struct w } : result :=
+  match check_model cls (w,m) with
+  | None => 
+    if is_model cls m then Model w m
+    else Unsatisfiable w m
+  | Some (w', v') => 
+    if LevelSet.equal w' V then Loop
+    else forward V cls v' w'
+  end.
+
+Definition mk_level x := LevelExpr.make (Level.Level x).
+Definition levela := mk_level "a".
+Definition levelb := mk_level "b".
+Definition levelc := mk_level "c".
+Definition leveld := mk_level "d".
+Definition levele := mk_level "e".
+
+Definition ex_levels : LevelSet.t := 
+  LevelSetProp.of_list (List.map (LevelExpr.get_level) [levela; levelb; levelc; leveld; levele]).
+
+Definition mk_clause (hd : LevelExpr.t) (premise : list LevelExpr.t) (e : LevelExpr.t) : clause := 
+  (NonEmptySetFacts.add_list premise (NonEmptySetFacts.singleton hd), e).
+
+Definition clause1 : clause := 
+  mk_clause levela [levelb] (LevelExpr.succ levelb).
+
+Definition levelexpr_add (x : LevelExpr.t) (n : nat) : LevelExpr.t :=
+  let (l, k) := x in (l, k + n).
+
+Definition clause2 : clause := mk_clause levelb [] (levelexpr_add levelc 3).
+Definition clause3 := mk_clause (levelexpr_add levelc 1) [] leveld.
+Definition clause4 := mk_clause levelb [levelexpr_add leveld 2] levele.
+Definition clause5 := mk_clause levele [] levela.
+
+Definition ex_clauses :=
+  ClausesProp.of_list [clause1; clause2; clause3; clause4].
+
+Definition ex_loop_clauses :=
+  ClausesProp.of_list [clause1; clause2; clause3; clause4; clause5].
+  
+Definition init_model (levels : LevelSet.t) : model :=
+  LevelSet.fold (fun l acc => LevelMap.add l 0 acc) levels (LevelMap.empty _).
+
+Definition init_w (levels : LevelSet.t) : LevelSet.t := LevelSet.empty.
+
+Example test := forward ex_levels ex_clauses (init_model ex_levels) (init_w ex_levels).
+Example test_loop := forward ex_levels ex_loop_clauses (init_model ex_levels) (init_w ex_levels).
+
+Eval compute in test.
+
+Definition print_model (m : model) :=
+  let list := LevelMap.elements m in
+  print_list (fun '(l, w) => string_of_level l ^ " -> " ^ string_of_nat w) nl list.
+
+Definition print_wset (l : LevelSet.t) :=
+  let list := LevelSet.elements l in
+  print_list string_of_level " " list.
+
+Definition print_result (m : result) :=
+  match m with
+  | Loop => "looping"
+  | Model w m => "satisfiable with model: " ^ print_model m ^ nl ^ " W = " ^
+    print_wset w
+  | Unsatisfiable w m => "Unsatisfiable with model: " ^ print_model m ^ " W = " ^ print_wset w
+  end.
+  
+Eval compute in print_result test.
+Eval compute in print_result test_loop.
+
+
+Definition clauses_of_constraint (cstr : UnivConstraint.t) : clauses :=
+  let '(l, d, r) := cstr in
+  match d with
+  | ConstraintType.Le k => 
+    (* Represent r >= lk + k <-> lk + k <= r *)
+    if (k <? 0)%Z then
+      let n := Z.to_nat (- k) in 
+      let r' := NonEmptySetFacts.map (fun l => levelexpr_add l n) r in
+        LevelExprSet.fold (fun lk acc => Clauses.add (r', lk) acc) l Clauses.empty
+    else
+      LevelExprSet.fold (fun lk acc => 
+        Clauses.add (r, levelexpr_add lk (Z.to_nat k)) acc) l Clauses.empty
+  | ConstraintType.Eq => 
+    let cls :=
+      LevelExprSet.fold (fun lk acc => Clauses.add (r, lk) acc) l Clauses.empty
+    in
+    let cls' :=
+      LevelExprSet.fold (fun rk acc => Clauses.add (l, rk) acc) r cls
+    in cls'
+  end.
+
+Definition clauses_of_constraints (cstrs : UnivConstraintSet.t) : clauses :=
+  UnivConstraintSet.fold (fun cstr acc => Clauses.union (clauses_of_constraint cstr) acc) cstrs Clauses.empty.
+
+Definition print_premise (l : LevelAlgExpr.t) : string :=
+  let (e, exprs) := LevelAlgExpr.exprs l in
+  string_of_level_expr e ^
+  match exprs with
+  | [] => "" 
+  | l => " \/ " ^ print_list string_of_level_expr " \/ " exprs 
+  end.
+
+Definition print_clauses (cls : clauses) :=
+  let list := Clauses.elements cls in
+  print_list (fun '(l, r) => 
+    print_premise l ^ " -> " ^ string_of_level_expr r) nl list.
